\documentclass{article}
\usepackage{ifthen}
\usepackage{epsfig}
\usepackage[utf8]{inputenc}
\usepackage{newunicodechar}
  \newunicodechar{⁻}{${}^{-}$}% Superscript minus
  \newunicodechar{²}{${}^{2}$}% Superscript two
  \newunicodechar{³}{${}^{3}$}% Superscript three

\pagestyle{empty}
\begin{document}
$ z(r)=\frac{r^2}{R\left( 1+\sqrt{1-(1+\kappa)\frac{r^2}{R^2}}\right)}+\sum_l\alpha_lr^l$
\pagebreak

$ z(r)=\frac{r^2}{R\left( 1+\sqrt{1-(1+\kappa)\frac{r^2}{R^2}}\right)}+\sum_l \alpha_l r^l $
\pagebreak

$fs^{-1}$
\pagebreak

$E(t)=E0 \cdot e^{-t^2/(2*\sigma^2)}$
\pagebreak

$\vec{E}(ar,z)=\vec{E}_0\frac{w_0}{w(z)}\cdot e^{\frac{r^2}{w^2(z)}}\cdot e^{-ik\frac{r^2}{2R(z)}}\cdot e^{i(\zeta(z)-kz)}$
\pagebreak

$ \frac{2\pi}{\lambda}$
\pagebreak

\[\frac{\Delta\lambda}{\lamda}=\frac{\Delta\omega}{\omega}\Rightarrow \Delta\omega=\Delta\lambda \cdot \frac{2\pi c}{\lambda^2}\]
\pagebreak

$-\frac{\pi}{2}$
\pagebreak

$-\pi$
\pagebreak

\end{document}
